Постройте доказательство в секвенциальном исчислении следующих высказываний:
\begin{enumcyr}
    \item $A \lor \lnot A$;
    \item $A \to \lnot \lnot A$ и $\lnot \lnot \lnot A \to \lnot A$;
    \item $((A \lor B) \to C) \to ((A \to C) \land (B \to C))$ и $((A \to C) \land (B \to C)) \to ((A \lor B) \to C)$;
    \item $((A \land C) \lor (B \land C)) \to ((A \lor B) \land C)$ и $((A \lor B) \land C) \to ((A \land C) \lor (B \land
	    C))$;
    \item $((A \lor C) \land (B \lor C)) \to ((A \land B) \lor C)$ и $((A \land B) \lor C) \to ((A \lor C) \lor	(B \lor C))$;
    \item $(\lnot B \to \lnot A) \to (A \to B)$.
\end{enumcyr}
